\documentclass[a4paper,12pt]{article}

\usepackage{amsmath}
\usepackage{times}

\newcommand{\D}{\mathrm{d}}

\begin{document}

Integrals with algebraic weights,
\begin{align*}
  I_{n}
  &=
  \int_{a}^{b}x^{n}(x-a)^{\mu-1}(b-x)^{\nu-1}\,\D x.    
\end{align*}

Using G\&R~3.196.3:
\begin{align*}
  \int_{a}^{b}(x-a)^{\mu-1}(b-x)^{\nu-1}\,\D x
  &=
    (b-a)^{\mu+\nu-1}B(\mu, \nu).
\end{align*}

Recursion relation. Consider
\begin{align*}
  J_{n} = \int_{a}^{b}
  x^{n} \frac{\D}{\D x}\left[(x-a)^{\mu}(b-x)^{\nu}\right]\,\D x.  
\end{align*}
Integrating by parts
\begin{align*}    
  J_{n} &=
    \left.
    x^{n}(x-a)^{\mu}(b-x)^{\nu}\right|_{a}^{b}\\
  &-
    n \int_{a}^{b}x^{n-1}(x-a)^{\mu}(b-x)^{\nu}\,\D x,\\
  &=
    n \int_{a}^{b}\left(x^{n+1} - (a+b)x^{n} + abx^{n-1}\right)
    (x-a)^{\mu-1}(b-x)^{\nu-1}\,\D x,\\
  &= nI_{n+1} - n(a+b)I_{n} + nabI_{n-1}.
\end{align*}
Evaluating the derivative,
\begin{align*}
  J_{n}
  &=
    \int_{a}^{b}x^{n}
    \left[
    b\mu + a\nu - (\mu+\nu)x
    \right]
    (x-a)^{\mu-1}(b-x)^{\nu-1}\,\D x,\\
  &= (b\mu + a\nu)I_{n} - (\mu+\nu)I_{n+1}.
\end{align*}
Equating,
\begin{align*}
  (n+\mu+\nu)I_{n+1}
  &=
    \left[
    n(a+b) + b\mu + a\nu
    \right]I_{n}
    -nab I_{n-1}.
\end{align*}

Recursion is seeded using,
\begin{align*}
  \int_{a}^{b}\frac{\D}{\D x}\left[(x-a)^{\mu}(b-x)^{\nu}\right]\,\D x
  &= 0,\\
  &= (b\mu + a\nu)I_{0} - (\mu+\nu)I_{1},
\end{align*}
giving
\begin{align*}
  I_{0} &= (b-a)^{\mu+\nu-1}B(\mu, \nu),\\
  I_{1} &= \frac{b\mu+a\nu}{\mu+\nu}I_{0}.
\end{align*}

\end{document}

%%% Local Variables:
%%% mode: latex
%%% TeX-master: t
%%% End:
